Merge reverse example into Arrays_Impl.

HOL/SepLogic/Arrays_Impl.thy
@@ -2,6 +2,8 @@ theory Arrays_Impl
   imports SepAuto "../DataStrs/Arrays_Ex"
 begin
 
+section {* Array copy *}
+
 fun array_copy :: "'a::heap array \<Rightarrow> 'a array \<Rightarrow> nat \<Rightarrow> unit Heap" where
   "array_copy a b 0 = (return ())"
 | "array_copy a b (Suc n) = do {
@@ -17,5 +19,49 @@ lemma array_copy_rule [hoare_triple]:
     array_copy a b n
    <\<lambda>_. a \<mapsto>\<^sub>a as * b \<mapsto>\<^sub>a Arrays_Ex.array_copy as bs n>"
 @proof @induct n @qed
+
+section {* Swap *}
+
+definition swap :: "'a::heap array \<Rightarrow> nat \<Rightarrow> nat \<Rightarrow> unit Heap" where [sep_proc]:
+  "swap a i j = do {
+     x \<leftarrow> Array.nth a i;
+     y \<leftarrow> Array.nth a j;
+     Array.upd i y a;
+     Array.upd j x a;
+     return ()
+   }"
+
+lemma swap_rule [hoare_triple]:
+  "i < length xs \<Longrightarrow> j < length xs \<Longrightarrow>
+   <p \<mapsto>\<^sub>a xs>
+   swap p i j
+   <\<lambda>_. p \<mapsto>\<^sub>a list_swap xs i j>" by auto2
+
+section {* Reverse *}
+
+fun rev :: "'a::heap array \<Rightarrow> nat \<Rightarrow> nat \<Rightarrow> unit Heap" where
+  "rev a i j = (if i < j then do {
+     swap a i j;
+     rev a (i + 1) (j - 1)
+   }
+   else return ())"
+declare rev.simps [sep_proc]
+
+lemma rev_to_fun [hoare_triple]:
+  "j < length xs \<Longrightarrow>
+   <p \<mapsto>\<^sub>a xs>
+   rev p i j
+   <\<lambda>_. p \<mapsto>\<^sub>a rev_swap xs i j>"
+@proof @fun_induct "rev_swap xs i j" @with
+  @subgoal "(xs = xs, i = i, j = j)"
+    @unfold "rev_swap xs i j"
+  @end
+@qed
+
+lemma rev_is_rev [hoare_triple]:
+  "xs \<noteq> [] \<Longrightarrow>
+   <p \<mapsto>\<^sub>a xs>
+   rev p 0 (length xs - 1)
+   <\<lambda>_. p \<mapsto>\<^sub>a List.rev xs>" by auto2
 
 end
